theories/tree_borrows/disjoint.v
@@ -1,0 +1,138 @@
+From simuliris.tree_borrows Require Import lang_base notation bor_semantics.
+
+Lemma create_child_isSome tr tgp tgc :
+  forall cids range tr' newp,
+  create_child cids tgp range tgc newp tr = Some tr' ->
+    (exists tr'', memory_read cids tgp range tr = Some tr''
+    /\ tr' = insert_child_at tr'' (create_new_item tgc newp range) (IsTag tgp)).
+Proof.
+  move=> ?? tr' ? CreateChild.
+  unfold create_child in CreateChild.
+  destruct (memory_read _ tgp _ tr); simpl in *; inversion CreateChild.
+  injection CreateChild; intros; subst.
+  exists t.
+  auto.
+Qed.
+
+Lemma item_apply_access_preserves_tag it :
+  forall kind cids rel range it',
+  item_apply_access kind cids rel range it = Some it' ->
+  itag it = itag it'.
+Proof.
+  move=> ???? it'.
+  unfold item_apply_access.
+  destruct (permissions_foreach _); simpl; [|intro H; inversion H].
+  intro H; injection H; intros; subst.
+  simpl; reflexivity.
+Qed.
+
+Lemma join_project_Exists {X} tr prop :
+  forall tr',
+  tree_join tr = Some tr' ->
+  tree_Exists prop tr' <-> tree_Exists (fun x => exists (v:X), x = Some v /\ prop v) tr.
+Proof.
+  induction tr; intros tr' JoinSome.
+  - simpl in JoinSome; injection JoinSome; intros; subst; tauto.
+  - simpl in JoinSome.
+    destruct data; simpl in *; [|inversion JoinSome].
+    destruct (tree_join tr1); simpl in *; [|inversion JoinSome].
+    destruct (tree_join tr2); simpl in *; [|inversion JoinSome].
+    injection JoinSome; intros; subst.
+    simpl.
+    split; intro H; destruct H as [H0 | [H1 | H2]].
+    * left. exists x; tauto.
+    * right; left. rewrite <- IHtr1; [exact H1|auto].
+    * right; right. rewrite <- IHtr2; [exact H2|auto].
+    * left. destruct H0 as [v [SomeV Pv]]; injection SomeV; intros; subst; auto.
+    * right; left. rewrite IHtr1; auto.
+    * right; right. rewrite IHtr2; auto.
+Qed.
+
+Lemma tree_Exists_increasing {X} (prop prop':Tprop X) tr :
+  tree_Exists prop tr ->
+  (forall x, prop x -> prop' x) ->
+  tree_Exists prop' tr.
+Proof.
+  induction tr; simpl; [tauto|].
+  intros H Impl; destruct H as [H0 | [H1 | H2]].
+  - left; apply Impl; auto.
+  - right; left; apply IHtr1; auto.
+  - right; right; apply IHtr2; auto.
+Qed.
+
+Lemma access_preserves_tags tr tg :
+  forall tr' app cids range rel,
+  tree_contains tg tr ->
+  tree_apply_access app cids tg range tr rel = Some tr' ->
+  tree_contains tg tr'.
+Proof.
+  move=> tr' app ??? Contains Access.
+  unfold tree_apply_access in Access.
+  unfold tree_contains in *.
+  rewrite join_project_Exists.
+  2: exact Access.
+  rewrite tree_Exists_map.
+  unfold compose.
+  apply (tree_Exists_increasing _ _ _ Contains).
+
+
+
+
+  generalize dependent tr'.
+  induction tr; [inversion Contains|].
+  intros tr' Access.
+  unfold tree_apply_access in *.
+  remember ( _ _ _ _ data) as newit.
+  remember (tree_join (tree_map _ tr1)) as new1.
+  remember (tree_join (tree_map _ tr2)) as new2.
+  destruct newit; simpl in Read; [|inversion Read].
+  destruct new1; simpl in Read; [|inversion Read].
+  destruct new2; simpl in Read; [|inversion Read].
+  injection Read; intros; subst.
+  destruct Contains as [C0 | [C1 | C2]].
+  - left.
+    unfold IsTag in *; subst.
+    symmetry in Heqnewit.
+    rewrite (item_apply_access_preserves_tag _ _ _ _ _ _ Heqnewit).
+    reflexivity.
+  - right; left.
+    symmetry in Heqnew1.
+    apply (IHtr1 _ _ _ _ Heqnew1).
+
+
+      + destruct (tree_join _); simpl in *; [|inversion H0].
+        injection H0; intros; subst.
+        destruct (item_apply_access _ _ _ _ data); simpl in *.
+        injection Read; intros; subst.
+
+  unfold memory_read in Read; unfold tree_apply_access in Read.
+
+
+Lemma new_item_has_tag tg :
+  forall perm range,
+  IsTag tg (create_new_item tg perm range).
+Proof.
+  move=> ??.
+  unfold create_new_item.
+  unfold IsTag; simpl; reflexivity.
+Qed.
+
+(* fresh t -> fresh t' -> insert t -> insert t' -> ~child t t' *)
+Lemma insertion_contains tr tgp tgc :
+  forall cids range tr' newp,
+  tree_contains tgp tr ->
+  create_child cids tgp range tgc newp tr = Some tr' ->
+  tree_contains tgc tr'.
+Proof.
+  move=> ?? tr' ? ContainsParent CreateChild.
+  unfold tree_contains in *.
+  destruct (create_child_isSome tr tgp tgc _ _ _ _ CreateChild) as [tr'' [Read Insert]].
+  rewrite Insert.
+  apply insert_True_produces_Exists.
+  - apply new_item_has_tag.
+  - 
+
+Lemma insertion_order_nonchild tr tg tg' :
+  ~tree_contains tg tr ->
+  ~tree_contains tg' tr ->
+
